theories/typing/empty.v
@@ -6,20 +6,25 @@ Implicit Type 𝔄 𝔅: syn_type.
 Section empty.
   Context `{!typeG Σ}.
 
-  Program Definition empty {𝔄} (n: nat) : type 𝔄 :=
-    {| pt_size := n; pt_own _ _ _ := False |}%I.
+  Program Definition empty {𝔄} : type 𝔄 :=
+    {| pt_size := 0; pt_own _ _ _ := False |}%I.
   Next Obligation. by iIntros. Qed.
 
-  Global Instance empty_empty : Empty (type ∅) := empty 0.
+  Global Instance empty_empty : Empty (type ∅) := empty.
 
-  Global Instance empty_send {𝔄} n : Send (@empty 𝔄 n). Proof. done. Qed.
+  Global Instance empty_send {𝔄} : Send (@empty 𝔄). Proof. done. Qed.
 
-  Lemma empty_subtype {𝔄 𝔅} (f: 𝔄 → 𝔅) n E L : subtype E L (empty n) (empty n) f.
+  Lemma empty_leak {𝔄} E L Φ : leak E L (@empty 𝔄) Φ.
+  Proof. by iIntros "* _ _ _ _" ([?[??]]). Qed.
+
+  Lemma empty_subtype {𝔄 𝔅} (f: 𝔄 → 𝔅) E L : subtype E L empty empty f.
   Proof.
     apply subtype_plain_type. iIntros "*_!>_/=". iSplit; [done|].
     iSplit; [iApply lft_incl_refl|by iIntros].
   Qed.
-  Lemma empty_eqtype {𝔄 𝔅} (f: 𝔄 → 𝔅) g n E L : eqtype E L (empty n) (empty n) f g.
+  Lemma empty_eqtype {𝔄 𝔅} (f: 𝔄 → 𝔅) g E L : eqtype E L empty empty f g.
   Proof. split; apply empty_subtype. Qed.
 
 End empty.
+
+Global Hint Resolve empty_leak empty_subtype empty_eqtype : lrust_typing.
